\input{../style/cs421_style.tex}
\usepackage{algorithm}
\usepackage{listings}
%\usepackage{algpseudocode}
\usepackage{graphicx,amssymb,amsmath}
\usepackage{epstopdf}
\sloppy

\oddsidemargin 0in
\evensidemargin 0in
\textwidth 6.5in
\topmargin -0.5in
\textheight 9.0in

\begin{document}

\newcommand\oversetSymbol[2]{\mathrel{\overset{\makebox[0pt]{\mbox{\normalfont\tiny\sffamily #2}}}{#1}}}

\def \betareduce { \xrightarrow{\beta} }
\def \alphaconvert { \xrightarrow{\alpha} }
\def \alphacongruent { \oversetSymbol{\sim}{\(\alpha\)} }

\solution{Dan McQuillan}{\today}{8}{Summer 2015}

\pagestyle{myheadings}  % Leave this command alone
	 	
\begin{enumerate}

	\def \proveL { ( \lambda y. x y ) ( \lambda x. \lambda y. y x) }
	\def \proveR { ( \lambda z. x z ) ( \lambda y. \lambda x. x y ) }

	\def \abstractionAL { \proveL }
	\def \abstractionAR { ( \lambda z. x z ) (\lambda x. \lambda x. \lambda y. y x) }
	\def \abstractionBL { \abstractionAR }
	\def \abstractionBR { ( \lambda z. x z ) ( \lambda w. \lambda y. y w ) }
	\def \abstractionCL { \abstractionBR }
	\def \abstractionCR { ( \lambda z. x z) ( \lambda w. \lambda x. x w ) }
	\def \abstractionDL  { \abstractionCR }
	\def \abstractionDR { \proveR }

	\item show: \( \proveL \alphacongruent \proveR  \)
	
	\begin{proof}
	\\
		\( \lambda y. x y \alphaconvert \lambda z. x z \) \hspace*{4mm} so: \\
		\( \lambda y. x y \alphaconvert \lambda z. x z \) \hspace*{4mm} so: \\
		\( \abstractionAL \alphacongruent \abstractionAR \) \\
		
		\( \lambda x. \lambda y. y x \alphaconvert \lambda w. \lambda y. y w \) \hspace*{4mm} so: \\
		\( \lambda x. \lambda y. y x \alphacongruent \lambda w. \lambda y. y w \) \hspace*{4mm} so: \\
		\( \abstractionBL \alphacongruent \abstractionBR \) \\
		
		\( \lambda w. \lambda y. y w \alphaconvert \lambda w. \lambda x. x w \) \hspace*{4mm} so: \\
		\( \lambda w. \lambda y. y w \alphacongruent \lambda w. \lambda x. x w \) \hspace*{4mm} so: \\
		\( \abstractionCL \alphacongruent \abstractionCR \) \\
		
		\( \lambda w. \lambda x. x w \alphaconvert \lambda y. \lambda x. x y \) \hspace*{4mm} so: \\
		\( \lambda w. \lambda x. x w \alphacongruent \lambda y. \lambda x. x y \) \hspace*{4mm} so: \\
		\( \abstractionDL \alphacongruent \abstractionDR \) \\
		
		Given the congruences above we know that:
		\begin{align}
			\abstractionAL {}& \alphacongruent \abstractionBL \\
					       {}& \alphacongruent \abstractionCL \\
					       {}& \alphacongruent \abstractionDL \\
					       {}& \alphacongruent \abstractionDR
		\end{align}
		
		By the transitive property we therefore know:
		\[
			\proveL \alphacongruent \proveR
		\]
	\end{proof}
	
	\item Evaluate \( ( \lambda x. x ( \lambda y. x y )) ((\lambda u. u) (\lambda w. w) ) \)
	
	\begin{enumerate}
		\item Eager Evaluation
		
		\begin{align}
			( \lambda x. x ( \lambda y. x y )) ((\lambda u. u) (\lambda w. w) ) {}& \rightarrow ( \lambda x. x ( \lambda y. x y )) ( \lambda w. w) \\
															 {}& \rightarrow ( \lambda w. w ) ( \lambda y. ( \lambda w. w ) y ) \\
															 {}& \rightarrow ( \lambda y. ( \lambda w. w ) y ) \\
															 {}& \rightarrow ( \lambda y. y ) 
		\end{align}
		
		\item Lazy Evaluation
		
		\begin{align}
			( \lambda x. x ( \lambda y. x y )) ((\lambda u. u) (\lambda w. w) ) {}& \rightarrow (( \lambda u. u) (\lambda w. w)) ( \lambda y. x y ) \\
															 {}& \rightarrow ( \lambda w. w) ( \lambda y. x y) \\
															 {}& \rightarrow ( \lambda y. x y )
		\end{align}
		
		\item unrestricted \( \alpha \beta \)-reduction
		
		\begin{align}
			( \lambda x. x ( \lambda y. x y )) ((\lambda u. u) (\lambda w. w) ) {}& \betareduce ( \lambda x. x ( \lambda y. x y )) ( \lambda w. w) \\
															 {}& \betareduce ( \lambda w. w) (\lambda y. ( \lambda w. w ) y ) \\
															 {}& \betareduce ( \lambda y. ( \lambda w. w ) y ) \\
															 {}& \betareduce ( \lambda y. y )
		\end{align}
	\end{enumerate}
\end{enumerate}

\end{document}

